\documentclass[11pt]{article}

\include{Header}

\begin{document}

\Submittedby{Breitenberger, Nicodemus}
\date{\today}

\section{Exercise 1}

\begin{lstlisting}

\end{lstlisting}

\section{Exercise 2}

\begin{lstlisting}

\end{lstlisting}

\section{Exercise 3}

\subsection{$ y''(x) + y(x) = \sin(2x) $}

General solution will be from the form $y(x) = y_c(x) + y_p(x)$, which is the sum of the complementary and particular solution.

First determine the complementary solution: 
\[ y''(x) + y(x) = 0 \]

Which can be solved by a sin(x) as well as a cos(x). Because 

\[  \partial^2_x \sin(x) = -\sin(x)  \]
\[  \partial^2_x \cos(x) = -\cos(x)  \]

Therefore

\[ y_c(x) = A\sin(x) + B\cos(x) \]

Second step is to determine the particular solution:

\[ y_p(x) = C\sin(2x) + D\cos(2x) \]
\[ \partial^2_x y_p(x) = -4C\sin(2x) -4D\cos(2x) \]

\[ -4C\sin(2x) -4D\cos(2x) + C\sin(2x) + D\cos(2x) = \sin(2x) \]
\[ -3C\sin(2x) - 3D\cos(2x) = \sin(2x) \]
\[ \Rightarrow D = 0 ~~~~ C = -\frac{1}{3}\sin(2x) \]

\[\boxed{ y(x) = A\sin(x) + B\cos(x) -\frac{1}{3}\sin(2x) }\]
Proof:
\[ y''(x) = -A\sin(x) - B\cos(x) -\frac{4}{3} \sin(2x)\]
\[ y''(x) + y(x) = \sin(x) + B\cos(x) -\frac{1}{3}\sin(2x) -A\sin(x) - B\cos(x) -\frac{4}{3} \sin(2x) = \sin(2x) \]

\subsection{$ y''(x) + y(x) = \sin(x) $}

Complementary solution same as in section 3.1.

\[ y_c(x) = A\sin(x) + B\cos(x) \]

Guess for particular solution:
\[ y_p(x) = C x \cos(x)\]
\[ y'_p(x) = C \cos(x) - C x \sin(x) \]
\[ y''_p(x) = - C \sin(x) - C x \cos(x) - C \sin(x) = -2 C \sin(x) - C x \cos(x) \]
\[ -2 C \sin(x) - C x \cos(x) + C x \cos(x) = \sin(x) \]
\[ \Rightarrow C = -\frac{1}{2} \]

\[\boxed{ y(x) = A\sin(x) + B\cos(x) -\frac{1}{2}x\cos(x) }\]

Proof:
\[ y''(x) = - A\sin(x) - B\cos(x) + \sin(x) - \frac{1}{2} x \cos(x) \]
\[ y''(x) + y(x) = A\sin(x) + B\cos(x) -\frac{1}{2}x\cos(x) - A\sin(x) - B\cos(x) + \sin(x) - \frac{1}{2} x \cos(x) \]
\[ = \sin(x) \]

\subsection{$ y''(x) - y(x) = 0 $}

This is a homogeneous differential equation. Therefore it is only necessary to find the homogeneous solution $y_c(x)$.

The equation can be solved by $e^x$ and $e^-x$. 

\[\boxed{ y(x) = Ae^x + Be^{-x} }\]  
Proof:

\[ y''(x) = Ae^x + (-1)^2Be^{-x} = Ae^x + Be^{-x}\]

\[ y''(x) - y(x) = Ae^x + Be^{-x} - Ae^x - Be^{-x} = 0\]
\end{document}
