\documentclass[11pt]{article}
\usepackage{bbold}
\include{Header}

\begin{document}

\Submittedby{Breitenberger, Nicodemus}
\date{\today}

\section{Exercise: Minimize RMSD}

\[ \textrm{RMSD}(A,B) = \min_{R,T} \sqrt{\frac{1}{N}\sum_i || A_i - R (B_i - T) ||^2 }\]

No rotation $\Rightarrow$ R is equal to identity matrix.

\[ \textrm{RMSD}(A,B) = \min_{T} \sqrt{\frac{1}{N}\sum_i || A_i - (B_i - T) ||^2 }\]

Minimize with respect to T $\Rightarrow \partial_T \textrm{RMSD}(A,B) = 0 $

\[ \partial_T \sqrt{\frac{1}{N}\sum_i || A_i - (B_i - T) ||^2} \]
\[ = \partial_T \sqrt{\frac{1}{N} \sum_i \left(\sqrt{\sum_i A_i - (B_i - T) }\right)^2} \]
\[ = \partial_T \sqrt{\frac{1}{N} \sum_i  A_i - (B_i - T)} = 0\]

\[ \Rightarrow T = \frac{1}{N} \sum_i (B_i - A_i) \]

This is equivalent to moving the center of mass of A into the center of mass of B.


\end{document}
