\documentclass[11pt]{article}

\include{Header}

\begin{document}

\Submittedby{Breitenberger, Nicodemus}
\date{\today}

\section{Exercise: Fourier transform}

\[ \begin{aligned}
	f_1(x) = \sin(x) &  &  x \in [-\pi,\pi] \\
	f_2(x) = \cos(x) &  &  x \in [-\pi,\pi] \\
	f_3(x) = e^{-x} &  &  x \in [0,2]
\end{aligned} \]

Fourier transformation:
\[ F[f](k) = \int_{-\infty}^{\infty} \frac{1}{\sqrt{2\pi}} f(x) e^{-ikx} dx \]

\[ F[f_1](k) = \int_{-\pi}^{\pi} \frac{1}{\sqrt{2\pi}} \sin(x) e^{-ikx} dx =  \frac{1}{\sqrt{2\pi}} \int_{-\pi}^{\pi} \frac{e^{ix}-e^{-ix}}{2i} e^{-ikx} dx \]
\[ = \frac{1}{\sqrt{2\pi}} \int_{-\pi}^{\pi} \frac{1}{2i} \left(e^{ix(1-k)} - e^{-ix(1+k)}\right) dx \]
\[ = \frac{1}{2i\sqrt{2\pi}} \left[\frac{1}{i(1-k)}e^{ix(1-k)} + \frac{1}{i(1+k)}e^{-ix(1+k)}\right]_{-\pi}^{\pi} \]
\[ = \frac{-1}{2\sqrt{2\pi}} \left[\frac{1}{(1-k)}e^{i\pi(1-k)} + \frac{1}{(1+k)}e^{-i\pi(1+k)} - \frac{1}{(1-k)}e^{i(-\pi)(1-k)} - \frac{1}{(1+k)}e^{-i(-\pi)(1+k)}\right]\]
\[ = \frac{-1}{2\sqrt{2\pi}}\frac{1}{(1 - k^2)} \left[(1+k)e^{i\pi(1-k)} + (1-k)e^{-i\pi(1+k)} - (1+k)e^{-i\pi(1-k)} - (1-k)e^{i\pi(1+k)}\right]\]
\[ = \frac{-1}{2\sqrt{2\pi}}\frac{1}{(1 - k^2)} \left[-(1+k)(e^{- i\pi k} - e^{i\pi k}) - (1-k)(e^{-i\pi k}  - e^{i\pi k})\right]\]
\[ = \frac{-1}{2\sqrt{2\pi}}\frac{1}{(1 - k^2)} \left[(- 1 - k - 1 + k)(e^{- i\pi k} - e^{i\pi k})\right]\]
\[ = \frac{-1}{2\sqrt{2\pi}}\frac{1}{(1 - k^2)} \left[-2 (e^{- i\pi k} - e^{i\pi k})\right] = \frac{1}{\sqrt{2\pi}}\frac{1}{(1 - k^2)} \left[ (e^{- i\pi k} - e^{i\pi k})\right]\]
\[ F[f_1](k) = \frac{-i}{(1 - k^2)}\sqrt{\frac{2}{\pi}} \sin(\pi k)\]

\newpage
\[ F[f_2](k) = \int_{-\pi}^{\pi} \frac{1}{\sqrt{2\pi}} \cos(x) e^{-ikx} dx =  \frac{1}{\sqrt{2\pi}} \int_{-\pi}^{\pi} \frac{e^{ix}+e^{-ix}}{2} e^{-ikx} dx \]
\[ = \frac{1}{2\sqrt{2\pi}} \int_{-\pi}^{\pi} \left(e^{ix(1-k)} + e^{-ix(1+k)}\right) dx \]
\[ = \frac{1}{2\sqrt{2\pi}} \left[\frac{1}{i(1-k)}e^{ix(1-k)} - \frac{1}{i(1+k)}e^{-ix(1+k)}\right]_{-\pi}^{\pi} \]
\[ = \frac{1}{2i\sqrt{2\pi}} \left[\frac{1}{(1-k)}e^{i\pi(1-k)} - \frac{1}{(1+k)}e^{-i\pi(1+k)} - \frac{1}{(1-k)}e^{-i\pi(1-k)} + \frac{1}{(1+k)}e^{i\pi(1+k)}\right] \]
\[ = \frac{1}{2i\sqrt{2\pi}}\frac{1}{(1-k^2)} \left[(1+k)e^{i\pi(1-k)} - (1-k)e^{-i\pi(1+k)} - (1+k)e^{-i\pi(1-k)} + (1-k)e^{i\pi(1+k)}\right] \]
\[ = \frac{1}{2i\sqrt{2\pi}}\frac{1}{(1-k^2)} \left[(1+k)(e^{i\pi(1-k)} - e^{-i\pi(1-k)}) + (1-k)(e^{i\pi(1+k)} - e^{-i\pi(1+k)})\right] \]
\[ = \frac{1}{2i\sqrt{2\pi}}\frac{1}{(1-k^2)} \left[-(1+k)(e^{-i\pi k} - e^{i\pi k}) + (1-k)(e^{-i\pi k} - e^{i\pi k})\right] \]
\[ = \frac{-2 k}{2i\sqrt{2\pi}}\frac{1}{(1-k^2)} (e^{-i\pi k} - e^{i\pi k}) = \frac{k}{(1-k^2)}\sqrt{\frac{2}{\pi}} \sin(\pi k) \]










\end{document}
